Adding CIMonadZero definition and making option an instance. Defining Simplicity with Assertions and its monadic semantics.

Coq/Simplicity/Alg.v
@@ -1,6 +1,9 @@
 Require Import Simplicity.Ty.
 Require Simplicity.Core.
+Require Simplicity.Assertion.
 Require Import Util.Monad.
+Require Import Util.Option.
+Let Hash256 := Simplicity.Assertion.Hash256.
 
 Set Implicit Arguments.
 Local Open Scope ty_scope.
@@ -20,13 +23,13 @@ Record class (term : Ty -> Ty -> Type) := Class
 ; take : forall {A B C}, term A C -> term (A * B) C
 ; drop : forall {A B C}, term B C -> term (A * B) C
 }.
+
 End Class.
 
 Structure Algebra := Pack { domain :> Ty -> Ty -> Type; class_of :> Class.class domain }.
 
-Record ReynoldsRel (alg1 alg2 : Algebra) :=
- { rel :> forall {A B}, alg1 A B -> alg2 A B -> Prop
- ; _ : forall A, rel (Class.iden alg1) (@Class.iden _ alg2 A)
+Record ReynoldsClass {alg1 alg2 : Algebra} (rel : forall {A B}, alg1 A B -> alg2 A B -> Prop) :=
+ { _ : forall A, rel (Class.iden alg1) (@Class.iden _ alg2 A)
  ; _ : forall A B C s1 s2 t1 t2, rel s1 s2 -> rel t1 t2 -> rel (Class.comp alg1 s1 t1) (@Class.comp _ alg2 A B C s2 t2)
  ; _ : forall A, rel (Class.unit alg1) (@Class.unit _ alg2 A)
  ; _ : forall A B C t1 t2, rel t1 t2 -> rel (Class.injl alg1 t1) (@Class.injl _ alg2 A B C t2)
@@ -35,6 +38,11 @@ Record ReynoldsRel (alg1 alg2 : Algebra) :=
  ; _ : forall A B C s1 s2 t1 t2, rel s1 s2 -> rel t1 t2 -> rel (Class.pair alg1 s1 t1) (@Class.pair _ alg2 A B C s2 t2)
  ; _ : forall A B C t1 t2, rel t1 t2 -> rel (Class.take alg1 t1) (@Class.take _ alg2 A B C t2)
  ; _ : forall A B C t1 t2, rel t1 t2 -> rel (Class.drop alg1 t1) (@Class.drop _ alg2 A B C t2)
+ }.
+
+Record ReynoldsRel (alg1 alg2 : Algebra) :=
+ { rel :> forall {A B}, alg1 A B -> alg2 A B -> Prop
+ ; reynoldsClass_of :> ReynoldsClass (@rel)
  }.
 
 Definition Reynolds {A B} (x y : forall (alg : Algebra), alg A B) : Prop :=
@@ -59,7 +67,7 @@ end.
 
 Lemma eval_Parametric {A B} (x : Simplicity.Core.Term A B) : Parametric (@eval A B x).
 Proof.
-intros alg1 alg2 [R].
+intros alg1 alg2 [R []].
 induction x; simpl; auto.
 Qed.
 
@@ -84,16 +92,15 @@ Qed.
 Lemma term_eval {A B} (x : forall alg : Algebra, alg A B) (Hx : Parametric x) (alg : Algebra) :
   x alg = eval (x Term).
 Proof.
-refine (Hx _ _ (Build_ReynoldsRel Term alg (fun a b x y => y = eval x) _ _ _ _ _ _ _ _ _));
+refine (Hx _ _ (@Build_ReynoldsRel Term alg (fun a b x y => y = eval x) _)); constructor;
 intros; simpl; congruence.
 Qed.
 
 End Term.
 
 End Core.
-
-Coercion Core.rel : Core.ReynoldsRel >-> Funclass.
 Coercion Core.domain : Core.Algebra >-> Funclass.
+Coercion Core.rel : Core.ReynoldsRel >-> Funclass.
 
 Section Core_Combinators.
 
@@ -111,7 +118,7 @@ Lemma iden_Parametric {alg1 alg2 : Core.Algebra} (R : Core.ReynoldsRel alg1 alg2
   {A} : R A A iden iden.
 Proof.
 unfold iden.
-destruct R as [R].
+destruct R as [R []].
 simpl; auto.
 Qed.
 
@@ -119,7 +126,7 @@ Lemma comp_Parametric {alg1 alg2 : Core.Algebra} (R : Core.ReynoldsRel alg1 alg2
   {A B C} s1 s2 t1 t2 : R A B s1 s2 -> R B C t1 t2 -> R A C (comp s1 t1) (comp s2 t2).
 Proof.
 unfold comp.
-destruct R as [R].
+destruct R as [R []].
 simpl; auto.
 Qed.
 
@@ -127,7 +134,7 @@ Lemma unit_Parametric {alg1 alg2 : Core.Algebra} (R : Core.ReynoldsRel alg1 alg2
   {A} : R A Unit unit unit.
 Proof.
 unfold unit.
-destruct R as [R].
+destruct R as [R []].
 simpl; auto.
 Qed.
 
@@ -135,7 +142,7 @@ Lemma injl_Parametric {alg1 alg2 : Core.Algebra} (R : Core.ReynoldsRel alg1 alg2
   {A B C} t1 t2 : R A B t1 t2 -> R A (B + C) (injl t1) (injl t2).
 Proof.
 unfold injl.
-destruct R as [R].
+destruct R as [R []].
 simpl; auto.
 Qed.
 
@@ -143,7 +150,7 @@ Lemma injr_Parametric {alg1 alg2 : Core.Algebra} (R : Core.ReynoldsRel alg1 alg2
   {A B C} t1 t2 : R A C t1 t2 -> R A (B + C) (injr t1) (injr t2).
 Proof.
 unfold injr.
-destruct R as [R].
+destruct R as [R []].
 simpl; auto.
 Qed.
 
@@ -151,7 +158,7 @@ Lemma case_Parametric {alg1 alg2 : Core.Algebra} (R : Core.ReynoldsRel alg1 alg2
   {A B C D} s1 s2 t1 t2 : R (A * C) D s1 s2 -> R (B * C) D t1 t2 -> R ((A + B) * C) D (case s1 t1) (case s2 t2).
 Proof.
 unfold case.
-destruct R as [R].
+destruct R as [R []].
 simpl; auto.
 Qed.
 
@@ -159,7 +166,7 @@ Lemma pair_Parametric {alg1 alg2 : Core.Algebra} (R : Core.ReynoldsRel alg1 alg2
   {A B C} s1 s2 t1 t2 : R A B s1 s2 -> R A C t1 t2 -> R A (B * C) (pair s1 t1) (pair s2 t2).
 Proof.
 unfold pair.
-destruct R as [R].
+destruct R as [R []].
 simpl; auto.
 Qed.
 
@@ -167,7 +174,7 @@ Lemma take_Parametric {alg1 alg2 : Core.Algebra} (R : Core.ReynoldsRel alg1 alg2
   {A B C} t1 t2 : R A C t1 t2 -> R (A * B) C (take t1) (take t2).
 Proof.
 unfold take.
-destruct R as [R].
+destruct R as [R []].
 simpl; auto.
 Qed.
 
@@ -175,7 +182,7 @@ Lemma drop_Parametric {alg1 alg2 : Core.Algebra} (R : Core.ReynoldsRel alg1 alg2
   {A B C} t1 t2 : R B C t1 t2 -> R (A * B) C (drop t1) (drop t2).
 Proof.
 unfold drop.
-destruct R as [R].
+destruct R as [R []].
 simpl; auto.
 Qed.
 
@@ -244,8 +251,9 @@ Notation "|[ x ]|^ M" := (x : Core.domain (CoreSem M) _ _) (at level 0, M at lev
 Notation "|[ x ]|" := (x : Core.domain CoreFunSem _ _) : core_alg_scope.
 
 Local Open Scope core_alg_scope.
+Local Open Scope monad_scope.
 
-Lemma CoreSem_natural {M A B} {x : forall {alg : Core.Algebra}, alg A B} (Hx : Core.Parametric (@x)) (a : A) :
+Lemma CoreSem_initial {M A B} {x : forall {alg : Core.Algebra}, alg A B} (Hx : Core.Parametric (@x)) (a : A) :
   |[ x ]|^M a = eta (|[ x ]| a).
 Proof.
 rewrite (Core.term_eval Hx (CoreSem M)).
@@ -264,4 +272,200 @@ induction t; cbn.
   apply phi_eta.
 - apply IHt.
 - apply IHt.
+Qed.
+
+Module Assertion.
+
+Module Class.
+
+Record mixin (term : Ty -> Ty -> Type) := Mixin
+{ assertl : forall {A B C D}, term (A * C) D -> Hash256 -> term ((A + B) * C) D
+; assertr : forall {A B C D}, Hash256 -> term (B * C) D -> term ((A + B) * C) D
+; fail : forall {A B}, (Hash256 * Hash256) -> term A B
+}.
+
+Record class (term : Ty -> Ty -> Type) := Class
+{ base : Core.Class.class term
+; ext  : mixin term
+}.
+
+End Class.
+Coercion Class.base : Class.class >-> Core.Class.class.
+Coercion Class.ext : Class.class >-> Class.mixin.
+
+Structure Algebra := Pack { domain :> Ty -> Ty -> Type; class_of :> Class.class domain }.
+
+Canonical Structure to_Core (alg : Algebra) : Core.Algebra := Core.Pack (class_of alg).
+
+Record ReynoldsMixin {alg1 alg2 : Algebra} (rel : forall {A B}, alg1 A B -> alg2 A B -> Prop) :=
+ { _ : forall A B C D s1 s2 th, rel s1 s2 -> rel (Class.assertl alg1 s1 th) (@Class.assertl _ alg2 A B C D s2 th)
+ ; _ : forall A B C D sh t1 t2, rel t1 t2 -> rel (Class.assertr alg1 sh t1) (@Class.assertr _ alg2 A B C D sh t2)
+ ; _ : forall A B hh, rel (Class.fail alg1 hh) (@Class.fail _ alg2 A B hh)
+ }.
+
+Record ReynoldsClass {alg1 alg2 : Algebra} (rel : forall {A B}, alg1 A B -> alg2 A B -> Prop) :=
+ { reynoldsBase :> Core.ReynoldsClass (@rel)
+ ; reynoldsExt :> ReynoldsMixin (@rel)
+ }.
+
+Record ReynoldsRel (alg1 alg2 : Algebra) :=
+ { rel :> forall {A B}, alg1 A B -> alg2 A B -> Prop
+ ; reynoldsClass_of :> ReynoldsClass (@rel)
+ }.
+
+Definition Reynolds {A B} (x y : forall (alg : Algebra), alg A B) : Prop :=
+  forall alg1 alg2 (R : ReynoldsRel alg1 alg2), R A B (x alg1) (y alg2).
+
+Definition Parametric {A B} (x : forall (alg : Algebra), alg A B) : Prop := Reynolds x x.
+
+Section Term.
+
+Fixpoint eval {A B} (x : Simplicity.Assertion.Term A B) {alg : Algebra} : alg A B :=
+match x in Simplicity.Assertion.Term A B return alg A B with
+| Simplicity.Assertion.iden => iden
+| Simplicity.Assertion.comp s t => comp (eval s) (eval t)
+| Simplicity.Assertion.unit => unit
+| Simplicity.Assertion.injl t => injl (eval t)
+| Simplicity.Assertion.injr t => injr (eval t)
+| Simplicity.Assertion.case s t => case (eval s) (eval t)
+| Simplicity.Assertion.pair s t => pair (eval s) (eval t)
+| Simplicity.Assertion.take t => take (eval t)
+| Simplicity.Assertion.drop t => drop (eval t)
+| Simplicity.Assertion.assertl s t => Class.assertl alg (eval s) t
+| Simplicity.Assertion.assertr s t => Class.assertr alg s (eval t)
+| Simplicity.Assertion.fail hh => Class.fail alg hh
+end.
+
+Lemma eval_Parametric {A B} (x : Simplicity.Assertion.Term A B) : Parametric (@eval A B x).
+Proof.
+intros alg1 alg2 [R [[] []]].
+induction x; simpl;
+unfold iden, comp, unit, injl, injr, case, pair, take, drop; auto.
+Qed.
+
+Canonical Structure Term_Core : Core.Algebra := Core.Pack (Core.Class.Class
+   Simplicity.Assertion.Term
+   (@Simplicity.Assertion.iden)
+   (@Simplicity.Assertion.comp)
+   (@Simplicity.Assertion.unit)
+   (@Simplicity.Assertion.injl)
+   (@Simplicity.Assertion.injr)
+   (@Simplicity.Assertion.case)
+   (@Simplicity.Assertion.pair)
+   (@Simplicity.Assertion.take)
+   (@Simplicity.Assertion.drop)).
+
+Canonical Structure Term : Algebra := @Pack Simplicity.Assertion.Term (Class.Class (Core.class_of Term_Core)
+  (Class.Mixin
+   Simplicity.Assertion.Term
+   (@Simplicity.Assertion.assertl)
+   (@Simplicity.Assertion.assertr)
+   (@Simplicity.Assertion.fail))
+  ).
+
+Lemma eval_Term {A B} (x : Simplicity.Assertion.Term A B) : eval x = x.
+Proof.
+induction x; unfold iden, comp, unit, injl, injr, case, pair, take, drop;
+cbn; congruence.
+Qed.
+
+Lemma term_eval {A B} (x : forall alg : Algebra, alg A B) (Hx : Parametric x) (alg : Algebra) :
+  x alg = eval (x Term).
+Proof.
+refine (Hx _ _ (@Build_ReynoldsRel Term alg (fun a b x y => y = eval x) _)); repeat constructor;
+intros; simpl; unfold iden, comp, unit, injl, injr, case, pair, take, drop;
+cbn; congruence.
+Qed.
+
+End Term.
+
+End Assertion.
+Coercion Assertion.domain : Assertion.Algebra >-> Funclass.
+Coercion Assertion.rel : Assertion.ReynoldsRel >-> Funclass.
+Coercion Assertion.Class.base : Assertion.Class.class >-> Core.Class.class.
+Coercion Assertion.Class.ext : Assertion.Class.class >-> Assertion.Class.mixin.
+Canonical Structure Assertion.to_Core.
+
+Section Assertion_Combinators.
+
+Definition assertl {A B C D} {alg : Assertion.Algebra} : alg (A * C) D -> Hash256 -> alg ((A + B) * C) D := Assertion.Class.assertl (Assertion.class_of alg).
+Definition assertr {A B C D} {alg : Assertion.Algebra} : Hash256 -> alg (B * C) D -> alg ((A + B) * C) D := Assertion.Class.assertr (Assertion.class_of alg).
+Definition fail {A B} {alg : Assertion.Algebra} : (Hash256 * Hash256) -> alg A B := Assertion.Class.fail (Assertion.class_of alg).
+
+Lemma assertl_Parametric {alg1 alg2 : Assertion.Algebra} (R : Assertion.ReynoldsRel alg1 alg2)
+  {A B C D} s1 s2 th : R (A * C) D s1 s2 -> R ((A + B) * C) D (assertl s1 th) (assertl s2 th).
+Proof.
+unfold assertl.
+destruct R as [R [Rb []]].
+simpl; auto.
+Qed.
+
+Lemma assertr_Parametric {alg1 alg2 : Assertion.Algebra} (R : Assertion.ReynoldsRel alg1 alg2)
+  {A B C D} sh t1 t2 : R (B * C) D t1 t2 -> R ((A + B) * C) D (assertr sh t1) (assertr sh t2).
+Proof.
+unfold assertr.
+destruct R as [R [Rb []]].
+simpl; auto.
+Qed.
+
+Lemma fail_Parametric {alg1 alg2 : Assertion.Algebra} (R : Assertion.ReynoldsRel alg1 alg2)
+  {A B} hh : R A B (fail hh) (fail hh).
+Proof.
+unfold assertr.
+destruct R as [R [Rb []]].
+simpl; firstorder.
+Qed.
+
+End Assertion_Combinators.
+
+Hint Resolve assertl_Parametric : parametricity.
+Hint Resolve assertr_Parametric : parametricity.
+Hint Immediate fail_Parametric : parametricity.
+
+Section AssertionSem.
+
+Definition AssertionSem_Mixin (M : CIMonadZero) := Assertion.Class.Mixin (Kleisli M)
+ (fun A B C D s _ p => let (ab, c) := p in
+    match ab with
+    | inl a => s (a, c)
+    | inr b => mzero
+    end)
+ (fun A B C D _ t p => let (ab, c) := p in
+    match ab with
+    | inl a => mzero
+    | inr b => t (b, c)
+    end)
+ (fun A B _ => kzero).
+
+Definition AssertionSem (M : CIMonadZero) : Assertion.Algebra :=
+  Assertion.Pack (Assertion.Class.Class (Core.class_of (CoreSem M)) (AssertionSem_Mixin M)).
+
+End AssertionSem.
+
+Notation "|[ x ]|^ M" := (x : Assertion.domain (AssertionSem M) _ _) (at level 0, M at level 0) : assertion_alg_scope.
+
+Local Open Scope assertion_alg_scope.
+
+(* TODO, try to replace option_Monad_Zero with just option *)
+Lemma AssertionSem_initial {M A B} {x : forall {alg : Assertion.Algebra}, alg A B} (Hx : Assertion.Parametric (@x)) (a : A) :
+  |[ x ]|^M a = optionZero (|[ x ]|^option_Monad_Zero a).
+Proof.
+repeat  rewrite (Assertion.term_eval Hx (AssertionSem _)).
+clear Hx.
+generalize (x Assertion.Term); clear x; intros t.
+induction t; cbn; try reflexivity.
+- symmetry; rewrite kleisli_comp_def.
+  rewrite optionZero_mu, optionZero_natural, map_comp, <- optionZero_natural, <- IHt1.
+  erewrite map_ext;[|intros;symmetry;apply IHt2].
+  rewrite <- kleisli_comp_def.
+  reflexivity.
+- rewrite IHt. apply optionZero_natural.
+- rewrite IHt; apply optionZero_natural.
+- destruct a as [[a|b] c]; [apply IHt1|apply IHt2].
+- rewrite IHt1, IHt2.
+  symmetry; apply optionZero_phi.
+- apply IHt.
+- apply IHt.
+- destruct a as [[a|b] c]; [apply IHt|reflexivity].
+- destruct a as [[a|b] c]; [reflexivity|apply IHt].
 Qed.
