Coq/Simplicity/Assertion.v
@@ -1,0 +1,52 @@
+Require Import Simplicity.Ty.
+Require Import Util.Monad.
+Require Import Util.Option.
+
+Variable Hash256 : Set (* TODO: Fill in suitable type for 256-bit word *).
+
+Local Open Scope monad_scope.
+
+Inductive Term : Ty -> Ty -> Set :=
+| iden : forall {A}, Term A A
+| comp : forall {A B C}, Term A B -> Term B C -> Term A C
+| unit : forall {A}, Term A Unit
+| injl : forall {A B C}, Term A B -> Term A (Sum B C)
+| injr : forall {A B C}, Term A C -> Term A (Sum B C)
+| case : forall {A B C D},
+    Term (Prod A C) D -> Term (Prod B C) D -> Term (Prod (Sum A B) C) D
+| pair : forall {A B C}, Term A B -> Term A C -> Term A (Prod B C)
+| take : forall {A B C}, Term A C -> Term (Prod A B) C
+| drop : forall {A B C}, Term B C -> Term (Prod A B) C
+| assertl : forall {A B C D},
+    Term (Prod A C) D -> Hash256 -> Term (Prod (Sum A B) C) D
+| assertr : forall {A B C D},
+    Hash256 -> Term (Prod B C) D -> Term (Prod (Sum A B) C) D
+| fail : forall {A B}, Hash256 * Hash256 -> Term A B.
+
+Fixpoint eval {A B} (x : Term A B) : tySem A -> option (tySem B) :=
+match x in Term A B return tySem A -> option (tySem B) with
+| iden => fun a => eta a
+| comp s t => fun a => (eval t <-< eval s) a
+| unit => fun _ => eta tt
+| injl t => fun a => map inl (eval t a)
+| injr t => fun a => map inr (eval t a)
+| case s t => fun p => let (ab, c) := p in
+    match ab with
+    | inl a => eval s (a, c)
+    | inr b => eval t (b, c)
+    end
+| pair s t => fun a => phi (eval s a) (eval t a)
+| take t => fun ab => eval t (fst ab)
+| drop t => fun ab => eval t (snd ab)
+| assertl s _ => fun p => let (ab, c) := p in
+    match ab with
+    | inl a => eval s (a, c)
+    | inr b => mzero
+    end
+| assertr _ t => fun p => let (ab, c) := p in
+    match ab with
+    | inl a => mzero
+    | inr b => eval t (b, c)
+    end
+| fail _ => kzero
+end.
