Simplicity-TR.tm
@@ -2439,7 +2439,7 @@
   The monad operations are defined as follows.
 
   <\eqnarray*>
-    <tformat|<table|<row|<cell|\<eta\><rsup|<maybe>><rsub|A><around*|(|a|)>>|<cell|\<assign\>>|<cell|<injr|<around*|(|a|)>>>>|<row|<cell|\<mu\><rsup|S><rsub|A><around*|(|<injl|<around*|\<langle\>||\<rangle\>>>|)>>|<cell|\<assign\>>|<cell|<injl|<around*|\<langle\>||\<rangle\>>>>>|<row|<cell|\<mu\><rsup|S><rsub|A><around*|(|<injr|<around*|(|<injl|<around*|\<langle\>||\<rangle\>>>|)>>|)>>|<cell|\<assign\>>|<cell|<injl|<around*|\<langle\>||\<rangle\>>>>>|<row|<cell|\<mu\><rsup|S><rsub|A><around*|(|<injr|<around*|(|<injr|<around*|(|a|)>>|)>>|)>>|<cell|\<assign\>>|<cell|<injr|<around*|(|a|)>>>>>>
+    <tformat|<table|<row|<cell|\<eta\><rsup|<maybe>><rsub|A><around*|(|a|)>>|<cell|\<assign\>>|<cell|<injr|<around*|(|a|)>>>>|<row|<cell|\<mu\><rsup|S><rsub|A><around*|(|<injl|<around*|\<langle\>||\<rangle\>>>|)>>|<cell|\<assign\>>|<cell|<injl|<around*|\<langle\>||\<rangle\>>>>>|<row|<cell|\<mu\><rsup|S><rsub|A><around*|(|<injr|<around*|(|x|)>>|)>>|<cell|\<assign\>>|<cell|x>>>>
   </eqnarray*>
 
   The option monad is commutative and idempotent. The option monad has a
